theories/Prelude/Memory.v
@@ -6,7 +6,7 @@ Definition val : Type := Z.
 Definition loc : Type := positive.
 
 (* [memory] is a mapping from location to a value *)
-Definition memory : Type := gmap loc val.
+Abbreviation memory := (gmap loc val).
 
 Definition loc_to_val (l: loc) : val := Zpos l.
 
@@ -23,11 +23,7 @@ Definition get_at (addr: val) (m: memory) : option val :=
 
 Definition update_at (addr: val) (f: val -> val) (m: memory) : option memory
   := match val_to_loc addr with
-     | Some loc =>
-         match m !! loc with
-         | Some old => Some (<[loc := f old]>m)
-         | None => None
-         end
+     | Some loc => Some (alter f loc m)
      | None => None
      end.
 
@@ -46,16 +42,44 @@ Qed.
 
 Lemma update_at_unfold : ∀ addr f m m',
   update_at addr f m = Some m' ->
-  ∃ l old,
-    val_to_loc addr = Some l ∧
-    m !! l = Some old ∧
-    <[l := f old]>m = m'.
+  ∃ loc,
+    val_to_loc addr = Some loc ∧
+    alter f loc m = m'.
 Proof using Type.
   intros addr f m m' H.
   unfold update_at in H.
   case_match eqn:Hloc; try congruence.
-  case_match eqn:Hmem; try congruence.
-  do 2 eexists. repeat split.
-  - eassumption.
+  eexists. split.
+  - reflexivity.
   - now inv H.
+Qed.
+
+Lemma alter_union_left f loc (m1 m2: memory) :
+  m1 ##ₘ m2 ->
+  m2 !! loc = None ->
+  alter f loc (m1 ∪ m2) = alter f loc m1 ∪ m2.
+Proof using Type.
+  intros Hdij Hnin.
+  unfold union, map_union.
+  rewrite (alter_union_with_l _ _ m1).
+  - reflexivity.
+  - intros x y H1 H2. exfalso.
+    rewrite map_disjoint_alt in Hdij.
+    destruct (Hdij loc) as [? | ?]; congruence.
+  - intros x H1 H2. congruence.
+Qed.
+
+Lemma alter_union_right f loc (m1 m2: memory) :
+  m1 ##ₘ m2 ->
+  m1 !! loc = None ->
+  alter f loc (m1 ∪ m2) = m1 ∪ alter f loc m2.
+Proof using Type.
+  intros Hdij Hnin.
+  unfold union, map_union.
+  rewrite (alter_union_with_r _ _ m1).
+  - reflexivity.
+  - intros x y H1 H2. exfalso.
+    rewrite map_disjoint_alt in Hdij.
+    destruct (Hdij loc) as [? | ?]; congruence.
+  - intros x H1 H2. congruence.
 Qed.
