theories/RTL/SimRules.v
@@ -1,4 +1,4 @@
-From RSL Require Import Prelude RelLogic.
+From RSL Require Import RelLogic Prelude.
 
 From Coinduction Require Import all.
 
@@ -20,54 +20,44 @@ Section Rules.
   Abbreviation fsim_lfp := (fsim_lfp WfNat WfNat Pₜ Pₛ).
   Abbreviation post := (val -> val -> rlogic).
 
-  Implicit Types C : Chain fsim_lfp.
-
-  Definition sim C Γ Φ fₜ pcₜ j i fₛ pcₛ : rlogic :=
+  Definition sim C ρ fₜ pcₜ j i fₛ pcₛ (Q: post) : rlogic :=
     let Φ : value Λₜ -> value Λₛ -> Prop :=
-      fun '(vₜ, mₜ) '(vₛ, mₛ) => Φ vₜ vₛ mₜ mₛ
+      fun '(vₜ, mₜ) '(vₛ, mₛ) => Q vₜ vₛ mₜ mₛ
     in
-    let '(ρₜ, ρₛ) := Γ in
+    let '(ρₜ, ρₛ) := ρ in
     fun mₜ mₛ =>
-      fsim_lfp (elem C) Φ
+      fsim_lfp C Φ
         j ([], State fₜ pcₜ ρₜ, mₜ)
         i ([], State fₛ pcₛ ρₛ, mₛ).
 
-  Notation
-    "C '|' Γ '⊢' ft '@' pct  '<{' j ',' i '}=' fs '@' pcs '{{' Φ '}}'" :=
-    (sim C Γ Φ%rlogic ft pct j i fs pcs)
-      (at level 1, ft at level 0, fs at level 0, no associativity).
-
-  Definition hoare C Γ P fₜ pcₜ j i fₛ pcₛ (Q: post) : Prop :=
-    ⊨ ∀ Φ,
-      P -*
-      (∀ vₜ vₛ, Q vₜ vₛ -* Φ vₜ vₛ) -*
-      sim C Γ Φ fₜ pcₜ j i fₛ pcₛ.
+  Definition hoare C ρ P fₜ pcₜ j i fₛ pcₛ Q : Prop :=
+    let '(ρₜ, ρₛ) := ρ in
+    emp ⊩ ∀ Φ, P -∗
+               (∀ vₜ vₛ, Q vₜ vₛ -∗ Φ vₜ vₛ) -∗
+               sim C ρ fₜ pcₜ j i fₛ pcₛ Φ.
 
   Notation
-    "C '|' Γ '⊢' '{{' P '}}' ft '@' pct  '<{' j ',' i '}=' fs '@' pcs '{{' Q '}}'" :=
-    (hoare C Γ P%rlogic ft pct j i fs pcs Q%rlogic)
-      (at level 1, ft at level 0, fs at level 0, no associativity).
+    "'[' C ']' ρ '⊢' ft '@' pct  '<{' j ',' i '}=' fs '@' pcs '{{' Q '}}'" :=
+    (sim C ρ ft pct j i fs pcs Q%rlogic)
+      (at level 0, ft at level 0, fs at level 0, no associativity).
 
   Notation
-    "C '|' Γ '⊢' '{{' '}}' ft '@' pct  '<{' j ',' i '}=' fs '@' pcs '{{' Q '}}'" :=
-    (hoare C Γ emp%rlogic ft pct j i fs pcs Q%rlogic)
-      (at level 1, ft at level 0, fs at level 0, no associativity).
+    "'[' C ']' ρ '⊢' '{{' P '}}' ft '@' pct  '<{' j ',' i '}=' fs '@' pcs '{{' Q '}}'" :=
+    (hoare C ρ P%rlogic ft pct j i fs pcs Q%rlogic)
+      (at level 0, ft at level 0, fs at level 0, no associativity).
 
-  Lemma both_ret C Γ (Φ: post)  fₜ pcₜ j i fₛ pcₛ :
+  Lemma both_ret C ρₜ ρₛ fₜ pcₜ j i fₛ pcₛ Q :
     ∀ rₜ vₜ rₛ vₛ,
     fₜ@pcₜ is <<{ ret rₜ }>> ->
     fₛ@pcₛ is <<{ ret rₛ }>> ->
-    Γ @ rₜ ⇒ₜ vₜ ->
-    Γ @ rₛ ⇒ₛ vₛ ->
-    C | Γ ⊢ {{ Φ vₜ vₛ }} fₜ @ pcₜ <{j, i}= fₛ @ pcₛ {{ Φ }}.
+    ρₜ @ rₜ ⇒ vₜ ->
+    ρₛ @ rₛ ⇒ vₛ ->
+    Q vₜ vₛ ⊩ [C] (ρₜ, ρₛ) ⊢ fₜ @ pcₜ <{j, i}= fₛ @ pcₛ {{ Q }}.
   Proof using Type.
     intros rt vt rs vs Hpct Hpcs Ht Hs.
-    intros Ψ mt1 ms1 ? ? Hpre mt2 ms2 ? ? Hpost.
+    intros mtQ msQ HQ.
 
-    simp. decompose_map_disjoint.
-    destruct Γ as [ρₜ ρₛ].
-    unfold rbank_assert_t, rbank_assert_t_single in Ht.
-    unfold rbank_assert_s, rbank_assert_s_single in Hs.
+    unfold regbank_assert, regbank_assert_single in *.
 
     eapply FSourceSteps with (i' := 0).
     { eapply exec_Iret; eassumption. }
@@ -80,46 +70,31 @@ Section Rules.
     eapply FRelated.
 
     do 2 eexists; repeat split. simpl.
-
-    rewrite (map_empty_union mt1).
-    rewrite (map_empty_union ms1).
-
-    erewrite (map_union_comm mt1 mt2) by eauto.
-    erewrite (map_union_comm ms1 ms2) by eauto.
-    apply Hpost.
-    - solve_map_disjoint.
-    - solve_map_disjoint.
-    - apply Hpre.
+    assumption.
   Qed.
 
-  Lemma source_nop C Γ Φ j fₜ pcₜ i fₛ pcₛ :
+  Lemma source_nop C ρₜ ρₛ P fₜ pcₜ j i fₛ pcₛ Q :
     ∀ pc,
     fₛ@pcₛ is <<{ nop -> pc }>> ->
-    C | Γ ⊢ {{ }} fₜ @ pcₜ <{j, 1+i}= fₛ @ pc {{ Φ }} ->
-    C | Γ ⊢ {{ }} fₜ @ pcₜ <{j, i}= fₛ @ pcₛ {{ Φ }}.
+    [C] (ρₜ, ρₛ) ⊢ {{ P }} fₜ @ pcₜ <{j, 1+i}= fₛ @ pc {{ Q }} ->
+    [C] (ρₜ, ρₛ) ⊢ {{ P }} fₜ @ pcₜ <{j, i}= fₛ @ pcₛ {{ Q }}.
   Proof using Type.
     intros pc Hpc H.
-    intros Ψ mt1 ms1 ? ? Hpre mt2 ms2 ? ? Hpost.
-
-    simp.
-    destruct Γ as [ρₜ ρₛ].
+    intros ? ? Hemp Ψ mtPre msPre ? ? Hpre mtPost msPost ? ? Hpost.
 
     eapply FSourceSteps.
     - econstructor; eassumption.
     - now apply H.
   Qed.
 
-  Lemma target_nop C Γ Φ j fₜ pcₜ i fₛ pcₛ :
+  Lemma target_nop C ρₜ ρₛ P fₜ pcₜ j i fₛ pcₛ Q :
     ∀ pc,
     fₜ@pcₜ is <<{ nop -> pc }>> ->
-    C | Γ ⊢ {{ }} fₜ @ pc <{1+j, i}= fₛ @ pcₛ {{ Φ }} ->
-    C | Γ ⊢ {{ }} fₜ @ pcₜ <{j, i}= fₛ @ pcₛ {{ Φ }}.
+    [C] (ρₜ, ρₛ) ⊢ {{ P }} fₜ @ pc <{1+j, i}= fₛ @ pcₛ {{ Q }} ->
+    [C] (ρₜ, ρₛ) ⊢ {{ P }} fₜ @ pcₜ <{j, i}= fₛ @ pcₛ {{ Q }}.
   Proof using Type.
     intros pc Hpc H.
-    intros Ψ mt1 ms1 ? ? Hpre mt2 ms2 ? ? Hpost.
-
-    simp.
-    destruct Γ as [ρₜ ρₛ].
+    intros ? ? Hemp Ψ mtPre msPre ? ? Hpre mtPost msPost ? ? Hpost.
 
     eapply FTargetSteps.
     - eexists. econstructor; eassumption.
@@ -127,39 +102,34 @@ Section Rules.
       eexists. now apply H.
   Qed.
 
-  Lemma source_op C Γ Φ j fₜ pcₜ i fₛ pcₛ :
+  Lemma source_op C ρₜ ρₛ P fₜ pcₜ j i fₛ pcₛ Q :
     ∀ pc dst op regs args v,
     fₛ@pcₛ is <<{ dst := @op regs -> pc }>> ->
+    ρₛ @ regs ⇒ args ->
     eval_op op args = Some v ->
-    Γ @ regs ⇒ₛ args ->
-    C | ⟦ dst ⇐ₛ v ⟧Γ ⊢ {{ }} fₜ @ pcₜ <{j, 1+i}= fₛ @ pc {{ Φ }} ->
-    C | Γ ⊢ {{  }} fₜ @ pcₜ <{j, i}= fₛ @ pcₛ {{ Φ }}.
+    [C] (ρₜ, ⟦dst ⇐ v⟧ρₛ) ⊢ {{ P }} fₜ @ pcₜ <{j, 1+i}= fₛ @ pc {{ Q }} ->
+    [C] (ρₜ, ρₛ) ⊢ {{ P }} fₜ @ pcₜ <{j, i}= fₛ @ pcₛ {{ Q }}.
   Proof using Type.
-    intros pc dst op regs args v Hpc Hv Hargs H.
-    intros Ψ mt1 ms1 ? ? Hpre mt2 ms2 ? ? Hpost.
-
-    simp.
-    destruct Γ as [ρₜ ρₛ].
+    intros pc dst op regs args v Hpc Hargs Hv H.
+    intros ? ? Hemp Ψ mtPre msPre ? ? Hpre mtPost msPost ? ? Hpost.
 
     eapply FSourceSteps.
     - econstructor; eassumption || reflexivity.
     - now eapply H.
   Qed.
 
-  Lemma target_op C Γ Φ j fₜ pcₜ i fₛ pcₛ :
+  Lemma target_op C ρₜ ρₛ P fₜ pcₜ j i fₛ pcₛ Q :
     ∀ pc dst op regs args v,
     fₜ@pcₜ is <<{ dst := @op regs -> pc }>> ->
+    ρₜ @ regs ⇒ args ->
     eval_op op args = Some v ->
-    Γ @ regs ⇒ₜ args ->
-    C | ⟦ dst ⇐ₜ v ⟧Γ ⊢ {{ }} fₜ @ pc <{1+j, i}= fₛ @ pcₛ {{ Φ }} ->
-    C | Γ ⊢ {{ }} fₜ @ pcₜ <{j, i}= fₛ @ pcₛ {{ Φ }}.
+    [C] (⟦dst ⇐ v⟧ρₜ, ρₛ) ⊢ {{ P }} fₜ @ pc <{1+j, i}= fₛ @ pcₛ {{ Q }} ->
+    [C] (ρₜ, ρₛ) ⊢ {{ P }} fₜ @ pcₜ <{j, i}= fₛ @ pcₛ {{ Q }}.
   Proof using Type.
-    intros pc dst op regs args v Hpc Hv Hargs H.
-    intros Ψ mt1 ms1 ? ? Hpre mt2 ms2 ? ? Hpost.
+    intros pc dst op regs args v Hpc Hargs Hv H.
+    intros ? ? Hemp Ψ mtPre msPre ? ? Hpre mtPost msPost ? ? Hpost.
 
-    simp.
-    destruct Γ as [ρₜ ρₛ].
-    unfold rbank_assert_t, rbank_assert_t_list in Hargs.
+    unfold regbank_assert, regbank_assert_list in *.
 
     eapply FTargetSteps.
     - eexists. econstructor; eassumption || reflexivity.
@@ -167,159 +137,161 @@ Section Rules.
       eexists. now apply H.
   Qed.
 
-  Lemma source_load C Γ Φ j fₜ pcₜ i fₛ pcₛ :
+  Lemma source_load C ρₜ ρₛ P fₜ pcₜ j i fₛ pcₛ Q :
     ∀ pc dst src addr v,
     fₛ@pcₛ is <<{ dst := !src -> pc }>> ->
-    Γ @ src ⇒ₛ addr ->
-    C | ⟦ dst ⇐ₛ v ⟧Γ ⊢ {{ addr →ₛ v }} fₜ @ pcₜ <{j, 1+i}= fₛ @ pc {{ Φ }} ->
-    C | Γ ⊢ {{ addr →ₛ v }} fₜ @ pcₜ <{j, i}= fₛ @ pcₛ {{ Φ }}.
+    ρₛ @ src ⇒ addr ->
+    [C] (ρₜ, ⟦dst ⇐ v⟧ρₛ) ⊢ {{ addr →ₛ v ∗ P }} fₜ @ pcₜ <{j, 1+i}= fₛ @ pc {{ Q }} ->
+    [C] (ρₜ, ρₛ) ⊢ {{ addr →ₛ v ∗ P }} fₜ @ pcₜ <{j, i}= fₛ @ pcₛ {{ Q }}.
   Proof using Type.
     intros pc dst src addr v Hpc Haddr H.
-    intros Ψ mt1 ms1 ? ? Hpre mt2 ms2 ? ? Hpost.
+    intros ? ? Hemp Ψ mtPre msPre ? ? Hpre mtPost msPost ? ? Hpost.
 
-    simp.
-    destruct Γ as [ρₜ ρₛ].
-    apply get_at_unfold in Hpre. destruct Hpre as (loc & Hloc & Hget).
+    destruct Hpre as (mtAddr & msAddr & mtP & msP & ? & ? & ? & ? & Hm & HP).
+    destruct Hm as (loc & Hloc & Hm).
 
     eapply FSourceSteps.
-    - eapply exec_Iload; try eassumption.
-      + unfold get_at. rewrite Hloc. simpl_map. reflexivity.
+    - eapply exec_Iload with (v := v); try eassumption.
+      + subst. decompose_map_disjoint.
+        unfold get_at. rewrite Hloc.
+        rewrite lookup_union_r, !lookup_union_l by easy.
+        apply lookup_singleton_eq.
       + reflexivity.
     - apply H; auto.
-      unfold get_at. now rewrite Hloc.
+      unfold rlogic_sep.
+      eexists mtAddr, msAddr, mtP, msP.
+      repeat split; auto.
+      eexists. split; eassumption.
   Qed.
 
-  Lemma target_load C Γ Φ j fₜ pcₜ i fₛ pcₛ :
+  Lemma target_load C ρₜ ρₛ P fₜ pcₜ j i fₛ pcₛ Q :
     ∀ pc dst src addr v,
     fₜ@pcₜ is <<{ dst := !src -> pc }>> ->
-    Γ @ src ⇒ₜ addr ->
-    C | ⟦ dst ⇐ₜ v ⟧Γ ⊢ {{ addr →ₜ v }} fₜ @ pc <{1+j, i}= fₛ @ pcₛ {{ Φ }} ->
-    C | Γ ⊢ {{ addr →ₜ v }} fₜ @ pcₜ <{j, i}= fₛ @ pcₛ {{ Φ }}.
+    ρₜ @ src ⇒ addr ->
+    [C] (⟦dst ⇐ v⟧ρₜ, ρₛ) ⊢ {{ addr →ₜ v ∗ P }} fₜ @ pc <{1+j, i}= fₛ @ pcₛ {{ Q }} ->
+    [C] (ρₜ, ρₛ) ⊢ {{ addr →ₜ v ∗ P }} fₜ @ pcₜ <{j, i}= fₛ @ pcₛ {{ Q }}.
   Proof using Type.
     intros pc dst src addr v Hpc Haddr H.
-    intros Ψ mt1 ms1 ? ? Hpre mt2 ms2 ? ? Hpost.
+    intros ? ? Hemp Ψ mtPre msPre ? ? Hpre mtPost msPost ? ? Hpost.
 
-    destruct Γ as [ρₜ ρₛ].
-    unfold rbank_assert_t, rbank_assert_t_single in Haddr.
-    apply get_at_unfold in Hpre.
-    destruct Hpre as (loc & Hloc & Hmem).
+    unfold regbank_assert, regbank_assert_single in Haddr.
+    destruct Hpre as (mtAddr & msAddr & mtP & msP & ? & ? & ? & ? & Hm & HP).
+    destruct Hm as (loc & Hloc & Hm).
 
     eapply FTargetSteps.
     - eexists. eapply exec_Iload; try eassumption.
-      + unfold get_at. rewrite Hloc. simpl_map. reflexivity.
+      + subst. decompose_map_disjoint.
+        unfold get_at. rewrite Hloc.
+        rewrite lookup_union_r, !lookup_union_l, lookup_singleton_eq by easy.
+        reflexivity.
       + reflexivity.
-    - intros t Hstep.
+    - subst. decompose_map_disjoint.
+      intros t Hstep.
       inv Hstep as [ | | | ? ? ? ? ? ? ? ? ? ? ? ? ? Hget | | | | | ].
+
       unfold get_at in Hget. rewrite Hloc in Hget.
-      simpl_map. inv Hget.
-      eexists. eapply H; auto. simp.
-      unfold get_at. now rewrite Hloc.
+      rewrite lookup_union_r, !lookup_union_l, lookup_singleton_eq
+                in Hget by easy.
+      injection Hget as <-.
+
+      eexists. apply H; try solve_map_disjoint.
+      eexists _, msAddr, mtP, msP. repeat split; eauto.
+      + solve_map_disjoint.
+      + exists loc. now split.
   Qed.
 
-  Lemma source_store C Γ Φ j fₜ pcₜ i fₛ pcₛ :
+  Lemma source_store C ρₜ ρₛ P fₜ pcₜ j i fₛ pcₛ Q :
     ∀ pc dst src addr v old,
     fₛ@pcₛ is <<{ !dst := src -> pc }>> ->
-    Γ @ dst ⇒ₛ addr ->
-    Γ @ src ⇒ₛ v ->
-    C | Γ ⊢ {{ addr →ₛ v }} fₜ @ pcₜ <{j, 1+i}= fₛ @ pc {{ Φ }} ->
-    C | Γ ⊢ {{ addr →ₛ old }} fₜ @ pcₜ <{j, i}= fₛ @ pcₛ {{ Φ }}.
+    ρₛ @ dst ⇒ addr ->
+    ρₛ @ src ⇒ v ->
+    [C] (ρₜ, ρₛ) ⊢ {{ addr →ₛ v ∗ P }} fₜ @ pcₜ <{j, 1+i}= fₛ @ pc {{ Q }} ->
+    [C] (ρₜ, ρₛ) ⊢ {{ addr →ₛ old ∗ P }} fₜ @ pcₜ <{j, i}= fₛ @ pcₛ {{ Q }}.
   Proof using Type.
     intros pc dst src addr v old Hpc Haddr Hv H.
-    intros Ψ mt1 ms1 ? ? Hpre mt2 ms2 ? ? Hpost.
+    intros ? ? Hemp Ψ mtPre msPre ? ? Hpre mtPost msPost ? ? Hpost.
 
-    simp.
-    destruct Γ as [ρₜ ρₛ].
-    apply get_at_unfold in Hpre. destruct Hpre as (l & Hloc & Hmem).
+    unfold regbank_assert, regbank_assert_single in Haddr, Hv.
+    destruct Hpre as (mtAddr & msAddr & mtP & msP & ? & ? & ? & ? & Hm & HP).
+    destruct Hm as (loc & Hloc & Hm).
 
     eapply FSourceSteps.
     - eapply exec_Istore; try eassumption.
+      subst. decompose_map_disjoint.
       unfold set_at, update_at. rewrite Hloc.
-      simpl_map.
-      rewrite (insert_union_l _ ms2).
-      rewrite (insert_union_r ∅ ms1).
-      + reflexivity.
-      + eapply map_disjoint_Some_l; eassumption.
-    - eapply H; auto.
-      + apply map_disjoint_insert_l. split; now eauto.
-      + unfold get_at. rewrite Hloc.
-        now rewrite (lookup_insert_eq ms1).
-      + decompose_map_disjoint.
-        apply map_disjoint_union_r. split; auto.
-        * solve_map_disjoint.
-        * apply map_disjoint_insert_r. split; eauto.
-          eapply map_disjoint_Some_r; eassumption.
+      rewrite alter_union_right, !alter_union_left, alter_singleton_eq;
+      solve_map_disjoint.
+
+    - subst. decompose_map_disjoint.
+      eapply H; try solve_map_disjoint.
+      eexists mtAddr, _, mtP, msP. repeat split; eauto.
+      + solve_map_disjoint.
+      + exists loc. now split.
   Qed.
 
-  Lemma target_store C Γ Φ j fₜ pcₜ i fₛ pcₛ :
+  Lemma target_store C ρₜ ρₛ P fₜ pcₜ j i fₛ pcₛ Q :
     ∀ pc dst src addr v old,
     fₜ@pcₜ is <<{ !dst := src -> pc }>> ->
-    Γ @ dst ⇒ₜ addr ->
-    Γ @ src ⇒ₜ v ->
-    C | Γ ⊢ {{ addr →ₜ v }} fₜ @ pc <{1+j, i}= fₛ @ pcₛ {{ Φ }} ->
-    C | Γ ⊢ {{ addr →ₜ old }} fₜ @ pcₜ <{j, i}= fₛ @ pcₛ {{ Φ }}.
+    ρₜ @ dst ⇒ addr ->
+    ρₜ @ src ⇒ v ->
+    [C] (ρₜ, ρₛ) ⊢ {{ addr →ₜ v ∗ P }} fₜ @ pc <{1+j, i}= fₛ @ pcₛ {{ Q }} ->
+    [C] (ρₜ, ρₛ) ⊢ {{ addr →ₜ old ∗ P }} fₜ @ pcₜ <{j, i}= fₛ @ pcₛ {{ Q }}.
   Proof using Type.
     intros pc dst src addr v old Hpc Haddr Hv H.
-    intros Ψ mt1 ms1 ? ? Hpre mt2 ms2 ? ? Hpost.
+    intros ? ? Hemp Ψ mtPre msPre ? ? Hpre mtPost msPost ? ? Hpost.
 
-    destruct Γ as [ρₜ ρₛ].
-    unfold rbank_assert_t, rbank_assert_t_single in Haddr, Hv.
-    apply get_at_unfold in Hpre. destruct Hpre as (l & Hloc & Hmem).
+    unfold regbank_assert, regbank_assert_single in Haddr, Hv.
+    destruct Hpre as (mtAddr & msAddr & mtP & msP & ? & ? & ? & ? & Hm & HP).
+    destruct Hm as (loc & Hloc & Hm).
 
     eapply FTargetSteps.
     - eexists. eapply exec_Istore; try eassumption.
-      unfold set_at, update_at. rewrite Hloc.
-      simpl_map. reflexivity.
+      unfold set_at, update_at. now rewrite Hloc.
     - intros t Hstep.
-      inv Hstep as [ | | | | ? ? ? ? ? ? ? ? ? ? ? ? ? ? Hm | | | | ].
-      unfold set_at, update_at in Hm. rewrite Hloc in Hm.
-      simpl_map.
-      rewrite (insert_union_l _ mt2) in Hm.
-      rewrite (insert_union_r ∅ mt1) in Hm by solve_map_disjoint.
-      inv Hm.
+      inv Hstep as [ | | | | ? ? ? ? ? ? ? ? ? ? ? ? ? ? Hset | | | | ].
 
-      eexists. simp. apply H; auto.
-      + apply map_disjoint_insert_l. split; now auto.
-      + unfold get_at. rewrite Hloc.
-        now rewrite (lookup_insert_eq mt1).
-      + decompose_map_disjoint.
-        apply map_disjoint_union_r. split; auto.
+      unfold set_at, update_at in Hset. rewrite Hloc in Hset.
+      rewrite alter_union_right, !alter_union_left, alter_singleton_eq
+                in Hset by solve_map_disjoint.
+      injection Hset as Hset.
+
+      subst. decompose_map_disjoint.
+      eexists. apply H; try solve_map_disjoint.
+      + eexists _, msAddr, mtP, msP. repeat split; eauto.
         * solve_map_disjoint.
-        * apply map_disjoint_insert_r. split; eauto.
-          eapply map_disjoint_Some_r; eassumption.
+        * exists loc. now split.
   Qed.
 
-  Lemma source_if C Γ Φ j fₜ pcₜ i fₛ pcₛ :
+  Lemma source_if C ρₜ ρₛ P fₜ pcₜ j i fₛ pcₛ Q :
     ∀ pc_true pc_false reg v pc,
     fₛ@pcₛ is <<{ if reg then goto pc_true else goto pc_false }>> ->
-    Γ @ reg ⇒ₛ v ->
+    ρₛ @ reg ⇒ v ->
     (if (v =? 0)%Z then pc_true else pc_false) = pc ->
-    C | Γ ⊢ {{ }} fₜ @ pcₜ <{j, 1+i}= fₛ @ pc {{ Φ }} ->
-    C | Γ ⊢ {{ }} fₜ @ pcₜ <{j, i}= fₛ @ pcₛ {{ Φ }}.
+    [C] (ρₜ, ρₛ) ⊢ {{ P }} fₜ @ pcₜ <{j, 1+i}= fₛ @ pc {{ Q }} ->
+    [C] (ρₜ, ρₛ) ⊢ {{ P }} fₜ @ pcₜ <{j, i}= fₛ @ pcₛ {{ Q }}.
   Proof using Type.
     intros pc_true pc_false reg v pc Hpc Hv Hnext_pc H.
-    intros Ψ ? ? ? ? Hpre ? ? ? ? Hpost. simp.
+    intros ? ? Hemp Ψ mtPre msPre ? ? Hpre mtPost msPost ? ? Hpost.
 
-    destruct Γ as [ρₜ ρₛ].
-    unfold rbank_assert_s, rbank_assert_s_single in Hv.
+    unfold regbank_assert, regbank_assert_single in Hv.
 
     eapply FSourceSteps.
     - econstructor; eassumption || reflexivity.
     - subst. now apply H.
   Qed.
 
-  Lemma target_if C Γ Φ j fₜ pcₜ i fₛ pcₛ :
+  Lemma target_if C ρₜ ρₛ P fₜ pcₜ j i fₛ pcₛ Q :
     ∀ pc_true pc_false reg v pc,
     fₜ@pcₜ is <<{ if reg then goto pc_true else goto pc_false }>> ->
-    Γ @ reg ⇒ₜ v ->
+    ρₜ @ reg ⇒ v ->
     (if (v =? 0)%Z then pc_true else pc_false) = pc ->
-    C | Γ ⊢ {{ }} fₜ @ pc <{j, i}= fₛ @ pcₛ {{ Φ }} ->
-    C | Γ ⊢ {{ }} fₜ @ pcₜ <{j, i}= fₛ @ pcₛ {{ Φ }}.
+    [C] (ρₜ, ρₛ) ⊢ {{ P }} fₜ @ pc <{1+j, i}= fₛ @ pcₛ {{ Q }} ->
+    [C] (ρₜ, ρₛ) ⊢ {{ P }} fₜ @ pcₜ <{j, i}= fₛ @ pcₛ {{ Q }}.
   Proof using Type.
     intros pc_true pc_false reg v pc Hpc Hv Hnext_pc H.
-    intros Ψ ? ? ? ? Hpre ? ? ? ? Hpost. simp.
+    intros ? ? Hemp Ψ mtPre msPre ? ? Hpre mtPost msPost ? ? Hpost.
 
-    destruct Γ as [ρₜ ρₛ].
-    unfold rbank_assert_t, rbank_assert_t_single in Hv.
+    unfold regbank_assert, regbank_assert_single in Hv.
 
     eapply FTargetSteps.
     - eexists. econstructor; eassumption || reflexivity.
@@ -327,81 +299,193 @@ Section Rules.
       eexists. now apply H.
   Qed.
 
-  Lemma frame C Γ Φ j fₜ pcₜ i fₛ pcₛ :
-    ∀ P Q,
-    C | Γ ⊢ {{ Q }} fₜ @ pcₜ <{j, i}= fₛ @ pcₛ {{ fun vₜ vₛ => Φ vₜ vₛ }} ->
-    C | Γ ⊢ {{ P ∗ Q }} fₜ @ pcₜ <{j, i}= fₛ @ pcₛ {{ fun vₜ vₛ => P ∗ Φ vₜ vₛ }}.
+  Lemma frame C ρₜ ρₛ P1 P2 fₜ pcₜ j i fₛ pcₛ Q :
+    [C] (ρₜ, ρₛ) ⊢ {{ P1 }} fₜ @ pcₜ <{j, i}= fₛ @ pcₛ {{ fun vₜ vₛ => Q vₜ vₛ }} ->
+    [C] (ρₜ, ρₛ) ⊢ {{ P1 ∗ P2 }} fₜ @ pcₜ <{j, i}= fₛ @ pcₛ {{ fun vₜ vₛ => Q vₜ vₛ ∗ P2 }}.
   Proof using Type.
-    intros P Q H.
-    intros Ψ mt2 ms2 ? ? Hpre mt3 ms3 ? ? Hpost.
-    decompose_map_disjoint.
+    intros H.
+    intros ? ? Hemp Ψ mtPre msPre ? ? Hpre mtPost msPost ? ? Hpost.
 
-    destruct Hpre as (mtP & mtQ & msP & msQ & ? & ? & ? & ? & Hp & Hq).
+    destruct Hpre as (mt1 & ms1 & mt2 & ms2 & ? & ? & ? & ? & HP1 & HP2).
+    subst. decompose_map_disjoint.
 
-    unfold hoare in H. simp.
+    rewrite (map_union_comm mt1 mt2) by easy.
+    rewrite (map_union_comm ms1 ms2) by easy.
 
-    rewrite (map_empty_union mt2).
-    rewrite (map_empty_union ms2).
+    rewrite <- (map_union_assoc mt2).
+    rewrite <- (map_union_assoc ms2).
+
+    rewrite (map_union_assoc mtPost mt2).
+    rewrite (map_union_assoc msPost ms2).
+
+    apply H; try solve_map_disjoint.
+
+    intros vₜ vₛ mt' ms' ? ? ?.
+    subst. decompose_map_disjoint.
+
+    rewrite (map_union_comm mtPost) by easy.
+    rewrite (map_union_comm msPost) by easy.
+
+    rewrite (map_union_assoc mt').
+    rewrite (map_union_assoc ms').
+
+    apply Hpost; try solve_map_disjoint.
+    exists mt', ms', mt2, ms2. repeat split; solve_map_disjoint.
+  Qed.
+
+  Lemma consequence C ρₜ ρₛ P fₜ pcₜ j i fₛ pcₛ Q :
+    ∀ P' Q',
+    (P ⊩ P') ->
+    (∀ vₜ vₛ, Q' vₜ vₛ ⊩ Q vₜ vₛ) ->
+    [C] (ρₜ, ρₛ) ⊢ {{ P' }} fₜ @ pcₜ <{j, i}= fₛ @ pcₛ {{ Q' }} ->
+    [C] (ρₜ, ρₛ) ⊢ {{ P }} fₜ @ pcₜ <{j, i}= fₛ @ pcₛ {{ Q }}.
+  Proof using Type.
+    intros P' Q' HP HQ H.
+    intros ? ? Hemp Ψ mtPre msPre ? ? Hpre mtPost msPost ? ? Hpost.
 
     subst. decompose_map_disjoint.
 
-    rewrite (map_union_comm mtP mtQ) by auto.
-    rewrite (map_union_comm msP msQ) by auto.
+    apply H; try solve_map_disjoint.
+    intros vₜ vₛ mt' ms' ? ? HQ'.
+    apply Hpost; auto.
+    now apply HQ.
+  Qed.
 
-    rewrite <- (map_union_assoc mtQ mtP mt3).
-    rewrite <- (map_union_assoc msQ msP ms3).
+  Local Lemma rewrite_hoare C ρₜ ρₛ P fₜ pcₜ j i fₛ pcₛ Q :
+    (
+      ∀ (Ψ: value Λₜ → value Λₛ → Prop) (mtP msP mtQ msQ : memory),
+        ∀ Φ,
+        (∀ vₜ vₛ mₜ mₛ, Φ vₜ vₛ mₜ mₛ <-> Ψ (vₜ, mₜ) (vₛ, mₛ)) ∧
+        mtP ##ₘ mtQ ∧
+        msP ##ₘ msQ ∧
+        P mtP msP ∧
+        (∀ (vₜ vₛ : val) (mt ms : memory),
+           mt ##ₘ mtQ ->
+           ms ##ₘ msQ ->
+           Q vₜ vₛ mt ms ->
+           Φ vₜ vₛ (mt ∪ mtQ) (ms ∪ msQ)
+        ) ->
+        fsim_lfp C (fun '(vₜ, mₜ) '(vₛ, mₛ) => Φ vₜ vₛ mₜ mₛ)
+          j ([], State fₜ pcₜ ρₜ, mtQ ∪ mtP)
+          i ([], State fₛ pcₛ ρₛ, msQ ∪ msP)
+    ) <->
+      [C] (ρₜ, ρₛ) ⊢ {{ P }} fₜ @ pcₜ <{j, i}= fₛ @ pcₛ {{ Q }}.
+  Proof using Type.
+    split; intros H.
+    - intros ? ? Hemp Ψ mtPre msPre ? ? Hpre mtPost msPost ? ? Hpost.
+      destruct Hemp as (-> & ->).
+      decompose_map_disjoint.
+      rewrite !(map_union_empty _).
+      apply H with (Ψ := fun '(vₜ, mₜ) '(vₛ, mₛ) => Ψ vₜ vₛ mₜ mₛ).
+      repeat split; easy.
+    - intros Ψ mtP msP mtQ msQ Φ (HΦ & Ht & Hs & Hpre & Hpost).
+      rewrite <- (map_union_empty mtP).
+      rewrite <- (map_union_empty msP).
+      apply H.
+      + now split.
+      + solve_map_disjoint.
+      + solve_map_disjoint.
+      + assumption.
+      + solve_map_disjoint.
+      + solve_map_disjoint.
+      + intros vₜ vₛ mt ms.
+        apply Hpost.
+  Qed.
 
-    rewrite <- (map_empty_union (mtQ ∪ (mtP ∪ mt3))).
-    rewrite <- (map_empty_union (msQ ∪ (msP ∪ ms3))).
-
-    rewrite ! (map_union_assoc ∅ _ _).
-
-    apply H.
+  Lemma coind ρₜ ρₛ Inv fₜ pcₜ j i fₛ pcₛ Q :
+    (∀ R ρₜ ρₛ,
+       (∀ ρₜ ρₛ j' i',
+          i < i' ->
+          j < j' ->
+          [R] (ρₜ, ρₛ) ⊢ {{ Inv ρₜ ρₛ }} fₜ @ pcₜ <{j', i'}= fₛ @ pcₛ {{ Q }}) ->
+       [R] (ρₜ, ρₛ) ⊢ {{ Inv ρₜ ρₛ }} fₜ @ pcₜ <{j, i}= fₛ @ pcₛ {{ Q }}
+    ) ->
+    [fsim] (ρₜ, ρₛ) ⊢ {{ Inv ρₜ ρₛ }} fₜ @ pcₜ <{j, i}= fₛ @ pcₛ {{ Q }}.
+  Proof using Type.
+    intros RIH.
+    rewrite <- rewrite_hoare.
+    intros Ψ mtP msP mtQ msQ Φ H.
+    apply fsim_unroll.
+    revert ρₜ ρₛ Ψ mtP msP mtQ msQ Φ H.
+    coinduction C CIH.
+    intros ρₜ ρₛ Ψ mtP msP mtQ msQ Φ (HΦ & Ht & Hs & Hpre & Hpost).
+    rewrite <- (map_union_empty mtP).
+    rewrite <- (map_union_empty msP).
+    apply RIH.
+    - intros ρₜ' ρₛ' j' i' Hi Hj.
+      rewrite <- rewrite_hoare.
+      repeat intro.
+      eapply FProgress.
+      { eassumption. }
+      { eassumption. }
+      eapply CIH. eassumption.
+    - now split.
     - solve_map_disjoint.
     - solve_map_disjoint.
     - assumption.
     - solve_map_disjoint.
     - solve_map_disjoint.
-    - intros vₜ vₛ mt' ms' ? ? ?.
-      subst. decompose_map_disjoint.
-
-      rewrite (map_union_comm mtP mt3) by auto.
-      rewrite (map_union_comm msP ms3) by auto.
-
-      rewrite <- (map_union_assoc mt3 mtP mt').
-      rewrite <- (map_union_assoc ms3 msP ms').
-
-      apply Hpost.
-      + solve_map_disjoint.
-      + solve_map_disjoint.
-      + do 4 eexists. repeat split.
-        * solve_map_disjoint.
-        * solve_map_disjoint.
-        * assumption.
-        * assumption.
+    - assumption.
   Qed.
 
-  Lemma consequence C Γ Φ j fₜ pcₜ i fₛ pcₛ :
-    ∀ P P' Φ',
-    (⊨ P -* P') ->
-    C | Γ ⊢ {{ P' }} fₜ @ pcₜ <{j, i}= fₛ @ pcₛ {{ Φ' }} ->
-    (∀ vₜ vₛ, ⊨ Φ' vₜ vₛ -* Φ vₜ vₛ) ->
-    C | Γ ⊢ {{ P }} fₜ @ pcₜ <{j, i}= fₛ @ pcₛ {{ Φ }}.
+  Lemma iex C ρₜ ρₛ fₜ pcₜ j i fₛ pcₛ Q :
+    ∀ T (P: T -> rlogic),
+    (∀ x,
+       [C] (ρₜ, ρₛ) ⊢ {{ P x }} fₜ @ pcₜ <{j, i}= fₛ @ pcₛ {{ Q }}) ->
+    [C] (ρₜ, ρₛ) ⊢ {{ ∃ x, P x }} fₜ @ pcₜ <{j, i}= fₛ @ pcₛ {{ Q }}.
   Proof using Type.
-    intros P P' Φ' HP H HΦ.
-    intros Ψ mt2 ms2 ? ? Hpre mt3 ms3 ? ? Hpost.
+    intros T P H.
+    intros ? ? Hemp Ψ mtPre msPre ? ? (x & Hpre).
+    eapply H.
+    - assumption.
+    - solve_map_disjoint.
+    - solve_map_disjoint.
+    - eassumption.
+  Qed.
 
-    simp. apply H; auto.
-    - rewrite <- (map_empty_union mt2).
-      rewrite <- (map_empty_union ms2).
-      apply HP; now auto.
-    - intros vₜ vₛ mt ms ? ? HΦ'.
-      apply Hpost; auto.
-      rewrite <- (map_empty_union mt).
-      rewrite <- (map_empty_union ms).
-      apply HΦ.
-      + solve_map_disjoint.
-      + solve_map_disjoint.
+  Lemma ipure C ρₜ ρₛ fₜ pcₜ j i fₛ pcₛ Q :
+    ∀ P1 P2,
+    (P1 -> [C] (ρₜ, ρₛ) ⊢ {{ P2 }} fₜ @ pcₜ <{j, i}= fₛ @ pcₛ {{ Q }})
+    <-> [C] (ρₜ, ρₛ) ⊢ {{ ⌜P1⌝ ∗ P2 }} fₜ @ pcₜ <{j, i}= fₛ @ pcₛ {{ Q }}.
+  Proof using Type.
+    intros P1 P2.
+    split.
+    - intros H.
+      intros ? ? Hemp Ψ mtPre msPre ? ? Hpre.
+      destruct Hpre as
+        (msP1 & mtP1 & mtP2 & msP2 & ? & ? & ? & ? & ((? & ?) & HP1) & HP2).
+      subst. decompose_map_disjoint.
+      eapply H.
       + assumption.
+      + assumption.
+      + solve_map_disjoint.
+      + solve_map_disjoint.
+      + now rewrite !(map_empty_union _).
+    - intros H HP1.
+      intros ? ? Hemp Ψ mtPre msPre ? ? Hpre.
+      eapply H.
+      + assumption.
+      + solve_map_disjoint.
+      + solve_map_disjoint.
+      + do 4 eexists. repeat split; eauto.
+        * solve_map_disjoint.
+        * solve_map_disjoint.
+        * apply map_empty_union.
+        * apply map_empty_union.
+  Qed.
+
+  Lemma index_mono (C: Chain fsim_lfp) ρₜ ρₛ P fₜ pcₜ j i fₛ pcₛ Q :
+    ∀ j' i',
+    (j' <= j)%nat ->
+    (i' <= i)%nat ->
+    [elem C] (ρₜ, ρₛ) ⊢ {{ P }} fₜ @ pcₜ <{j', i'}= fₛ @ pcₛ {{ Q }} ->
+    [elem C] (ρₜ, ρₛ) ⊢ {{ P }} fₜ @ pcₜ <{j, i}= fₛ @ pcₛ {{ Q }}.
+  Proof using Type.
+    intros i' j' Hi Hj H.
+    intros ? ? Hemp Ψ mtPre msPre ? ? Hpre mtPost msPost ? ? Hpost.
+    eapply idx_mono.
+    - now apply H.
+    - unfold "⊑". simpl. lia.
+    - unfold "⊑". simpl. lia.
   Qed.
 End Rules.
