theories/RelLogic/Logic.v
@@ -19,15 +19,15 @@ Section LogicOp.
   Definition rlogic_and (P Q: rlogic) : rlogic :=
     fun mt ms => P mt ms ∧ Q mt ms.
 
-  Definition rlogic_sep_and (P Q: rlogic) : rlogic :=
+  Definition rlogic_sep (P Q: rlogic) : rlogic :=
     fun mt ms =>
-      ∃ mt1 mt2 ms1 ms2,
-        mt1 ##ₘ mt2 ∧
-        ms1 ##ₘ ms2 ∧
-        mt1 ∪ mt2 = mt ∧
-        ms1 ∪ ms2 = ms ∧
-        P mt1 ms1 ∧
-        Q mt2 ms2.
+      ∃ mtP msP mtQ msQ,
+        mtP ##ₘ mtQ ∧
+        msP ##ₘ msQ ∧
+        mtP ∪ mtQ = mt ∧
+        msP ∪ msQ = ms ∧
+        P mtP msP ∧
+        Q mtQ msQ.
 
   Definition rlogic_or (P Q: rlogic) : rlogic :=
     fun mt ms => P mt ms ∨ Q mt ms.
@@ -37,29 +37,32 @@ Section LogicOp.
 
   Definition rlogic_wand (P Q: rlogic) : rlogic :=
     fun mt ms =>
-      ∀ mt' ms',
-      mt' ##ₘ mt ->
-      ms' ##ₘ ms ->
-      P mt' ms' ->
-      Q (mt ∪ mt') (ms ∪ ms').
+      ∀ mtP msP,
+      mtP ##ₘ mt ->
+      msP ##ₘ ms ->
+      P mtP msP ->
+      Q (mtP ∪ mt) (msP ∪ ms).
 
   Definition rlogic_not (P: rlogic) : rlogic :=
     fun mt ms => ~ P mt ms.
 
-  Definition rlogic_exists {X: Type} (f: X -> rlogic) : rlogic :=
+  Definition rlogic_exist {X: Type} (f: X -> rlogic) : rlogic :=
     fun mt ms => ∃ x, f x mt ms.
 
   Definition rlogic_forall {X: Type} (f: X -> rlogic) : rlogic :=
     fun mt ms => ∀ x, f x mt ms.
 
-  Definition rlogic_pure (P: Prop) : rlogic :=
-    fun mt ms => mt = ∅ ∧ ms = ∅ ∧ P.
-
   Definition rlogic_empty : rlogic :=
     fun mt ms => mt = ∅ ∧ ms = ∅.
 
-  Definition rlogic_entails (P: rlogic) : Prop :=
-    P ∅ ∅.
+  Definition rlogic_pure (P: Prop) : rlogic :=
+    fun mt ms => rlogic_empty mt ms ∧ P.
+
+  Definition rlogic_entails (P Q: rlogic) : Prop :=
+    ∀ mt ms, P mt ms -> Q mt ms.
+
+  Definition rlogic_all_memory : rlogic :=
+    fun _ _ => True.
 
 End LogicOp.
 
@@ -68,20 +71,17 @@ Notation "x ∧ y" :=
     (at level 80, y constr at level 80, right associativity) : rlogic_scope.
 
 Notation "x ∗ y" :=
-  (rlogic_sep_and x y)
+  (rlogic_sep x y)
     (at level 80, y constr at level 80, right associativity) : rlogic_scope.
 
 Notation "x ∨ y" :=
   (rlogic_or x y)
     (at level 85, y constr at level 85, right associativity) : rlogic_scope.
 
-Notation "x → y" := (rlogic_impl x y)
-  (at level 99, y at level 200, right associativity) : rlogic_scope.
-
 Notation "x -> y" := (rlogic_impl x y)
   (at level 99, y at level 200, right associativity) : rlogic_scope.
 
-Notation "x -* y" := (rlogic_wand x y)
+Notation "x -∗ y" := (rlogic_wand x y)
   (at level 99, y at level 200, right associativity) : rlogic_scope.
 
 Notation "~ x" :=
@@ -98,7 +98,7 @@ Notation "∀ x .. y , P" :=
      format "'[ ' '[ ' ∀ x .. y ']' , '/' P ']'") : rlogic_scope.
 
 Notation "∃ x .. y , P" :=
-  (rlogic_exists (fun x => .. (rlogic_exists (fun y => P)) ..))
+  (rlogic_exist (fun x => .. (rlogic_exist (fun y => P)) ..))
     (at level 10, x binder, y binder, P at level 200,
      format "'[ ' '[ ' ∃ x .. y ']' , '/' P ']'") : rlogic_scope.
 
@@ -108,75 +108,81 @@ Notation "⌜ P ⌝" :=
 Notation "⦇ P ⦈" :=
   (P)%rlogic (at level 0, P at level 200, format "⦇ P ⦈").
 
-Notation "⊨ P" :=
-  (rlogic_entails P%rlogic) (at level 99, right associativity).
+Notation "P ⊩ Q" :=
+  (rlogic_entails P%rlogic Q%rlogic) (at level 99, right associativity).
 
 Notation "⌜⌝" := (rlogic_empty) (at level 0) : rlogic_scope.
 
-Global Abbreviation emp := (rlogic_empty).
+Abbreviation emp := (rlogic_empty).
 
-(** ** Memory Connectives *)
+Abbreviation GC := (rlogic_all_memory).
 
-Section MemoryOp.
-  Definition rlogic_mem_t_assert addr v : rlogic :=
-    fun mt _ => get_at addr mt = Some v.
+Lemma add_true_l P :
+  P ⊩ P ∗ ⌜⌝.
+Proof.
+  intros mt ms HP.
+  exists mt, ms, ∅, ∅. repeat split.
+  - apply map_disjoint_empty_r.
+  - apply map_disjoint_empty_r.
+  - apply map_union_empty.
+  - apply map_union_empty.
+  - assumption.
+Qed.
 
-  Definition rlogic_mem_s_assert addr v : rlogic :=
-    fun _ ms => get_at addr ms = Some v.
+Lemma add_true_r P :
+  P ⊩ ⌜⌝ ∗ P.
+Proof.
+  intros mt ms HP.
+  exists ∅, ∅, mt, ms. repeat split.
+  - apply map_disjoint_empty_l.
+  - apply map_disjoint_empty_l.
+  - apply map_empty_union.
+  - apply map_empty_union.
+  - assumption.
+Qed.
 
-  Definition rlogic_mem_same_at P addrt addrs : rlogic :=
-    fun mt ms =>
-      P (get_at addrt mt) (get_at addrs ms).
+Lemma remove_true_l P :
+  P ∗ ⌜⌝ ⊩ P.
+Proof.
+  intros mt ms HP.
+  destruct HP as (mtP & msP & ? & ? & ? & ? & <- & <- & HP & Hemp).
+  destruct Hemp as [-> ->].
+  rewrite !(map_union_empty _).
+  assumption.
+Qed.
 
-End MemoryOp.
+Lemma entails_refl P :
+  P ⊩ P.
+Proof.
+  now intros mt ms HP.
+Qed.
 
-Notation "l '→ₜ' v" :=
-  (rlogic_mem_t_assert l%positive v%Z)
-    (at level 70, no associativity, format "l →ₜ v") : rlogic_scope.
+Global Instance entails_refl_inst : Reflexive rlogic_entails := entails_refl.
 
-Notation "l '→ₛ' v" :=
-  (rlogic_mem_s_assert l%positive v%Z)
-    (at level 70, no associativity, format "l →ₛ v") : rlogic_scope.
+Lemma sep_comm P Q :
+  P ∗ Q ⊩ Q ∗ P.
+Proof.
+  intros mt ms (mtP & msP & mtQ & msQ & Ht & Hs & Hcupt & Hcups & HP & HQ).
+  subst.
+  exists mtQ, msQ, mtP, msP.
+  repeat split.
+  - solve_map_disjoint.
+  - solve_map_disjoint.
+  - apply map_union_comm. solve_map_disjoint.
+  - apply map_union_comm. solve_map_disjoint.
+  - assumption.
+  - assumption.
+Qed.
 
-Notation "addrt 'ₜ⟨' P '⟩ₛ' addrs" :=
-  (rlogic_mem_same_at P addrt%positive addrs%positive)
-    (at level 70, no associativity) : rlogic_scope.
-
-Notation "addrs 'ₛ⟨' P '⟩ₜ' addrt" :=
-  (rlogic_mem_same_at P addrt%positive addrs%positive)
-    (at level 70, no associativity) : rlogic_scope.
-
-Notation "addrt 'ₜ~ₛ' addrs" :=
-  (rlogic_mem_same_at eq addrt%positive addrs%positive)
-    (at level 70, no associativity) : rlogic_scope.
-
-Notation "addrs 'ₛ~ₜ' addrt" :=
-  (rlogic_mem_same_at eq addrt%positive addrs%positive)
-    (at level 70, no associativity) : rlogic_scope.
-
-(** ** Auto unfolding *)
-
-Create HintDb custom_rlogic discriminated.
-
-Hint Unfold
-  rlogic_and
-  rlogic_sep_and
-  rlogic_or
-  rlogic_impl
-  rlogic_wand
-  rlogic_not
-  rlogic_exists
-  rlogic_forall
-
-  rlogic_pure
-  rlogic_empty
-  rlogic_entails
-
-  rlogic_mem_t_assert
-  rlogic_mem_s_assert
-  rlogic_mem_same_at
-  : custom_rlogic.
-
-Ltac simp :=
-  autounfold with custom_rlogic in *;
-  cbn beta iota zeta delta in *.
+Lemma sep_pure_left P Q :
+  P -> Q ⊩ ⌜P⌝ ∗ Q.
+Proof.
+  intros HP mt ms HQ.
+  exists ∅, ∅, mt, ms. repeat split.
+  - solve_map_disjoint.
+  - solve_map_disjoint.
+  - apply map_empty_union.
+  - apply map_empty_union.
+  - assumption.
+  - assumption.
+Qed.
